rocq/Ender/Parser.v
@@ -503,6 +503,8 @@ Definition parse_reason_chars (raw : chars) : option Reason :=
         (try_call "pgram_opp_sides" text (parse_one PgramOppSides)
         (try_call "pgram_opp_angs" text (parse_one PgramOppAngles)
         (try_call "pgram_consec_angs" text (parse_one PgramConsecAngs)
+        (try_call "pgram_opp_sides_conv" text (parse_two PgramOppSidesConv)
+        (try_call "rect_pgram_ang" text (parse_two RectPgramAng)
         (try_call "pgram_opp_side_para" text (parse_two PgramOppSidePara)
         (try_call "rectangle_pgram" text (parse_one RectanglePgram)
         (try_call "rhombus_pgram" text (parse_one RhombusPgram)
@@ -524,7 +526,7 @@ Definition parse_reason_chars (raw : chars) : option Reason :=
         (try_call "inscribed_semi" text (parse_one InscribedSemi)
         (try_call "con_chords_intersect_arcs" text (parse_one ConChordsArcs)
         (try_call "tangent_perp" text (parse_two TangentPerp)
-        None)))))))))))))))))))))))))))))))))))))))))))))))))))))))
+        None)))))))))))))))))))))))))))))))))))))))))))))))))))))))))
     end
   end.
 
