rocq/Ender/Syntax.v
@@ -97,6 +97,8 @@ Inductive Reason :=
 | PgramOppSides : nat -> Reason
 | PgramOppAngles : nat -> Reason
 | PgramConsecAngs : nat -> Reason
+| PgramOppSidesConv : nat -> nat -> Reason
+| RectPgramAng : nat -> nat -> Reason
 | PgramOppSidePara : nat -> nat -> Reason
 | RectanglePgram : nat -> Reason
 | RhombusPgram : nat -> Reason
